remove Balloc.rep from Inode.rep

src/Inode.v
@@ -451,9 +451,8 @@ Module INODE.
     [[ IBlocks ino = firstn (length (IBlocks ino)) ((ino' :-> "blocks") ++ blist) ]]
     )%pred.
 
-  Definition rep bxp xp (ilist : list inode) := (
-     exists ilist' freelist, 
-     rep' xp ilist' * BALLOC.rep bxp freelist *
+  Definition rep xp (ilist : list inode) := (
+     exists ilist', rep' xp ilist' *
      listmatch inode_match ilist ilist')%pred.
 
   Definition inode_match_direct ino (ino' : inode') : @pred addrlen valu := (
@@ -623,8 +622,8 @@ Module INODE.
   Hint Rewrite resolve_selN_valu0   using reflexivity : defaults.
 
 
-  Lemma rep_bound: forall F bxp xp l m,
-    (F * rep bxp xp l)%pred m
+  Lemma rep_bound: forall F xp l m,
+    (F * rep xp l)%pred m
     -> length l <= wordToNat (IXLen xp ^* items_per_valu).
   Proof.
     unfold rep, rep'; intros.
@@ -632,8 +631,8 @@ Module INODE.
     erewrite listmatch_length_r; eauto; omega.
   Qed.
 
-  Lemma blocks_bound: forall F bxp xp l m i,
-    (F * rep bxp xp l)%pred m
+  Lemma blocks_bound: forall F xp l m i,
+    (F * rep xp l)%pred m
     -> length (IBlocks (sel l i inode0)) <= wordToNat (natToWord addrlen blocks_per_inode).
   Proof.
     unfold rep, sel; intros.
@@ -688,9 +687,9 @@ Module INODE.
   Hint Extern 0 (okToUnify (indrep _ _) (indrep _ _)) => constructor : okToUnify.
 
   Theorem ilen_ok : forall lxp xp inum ms,
-    {< F A mbase m ilist ino bxp,
+    {< F A mbase m ilist ino,
     PRE    MEMLOG.rep lxp (ActiveTxn mbase m) ms *
-           [[ (F * rep bxp xp ilist)%pred (list2mem m) ]] *
+           [[ (F * rep xp ilist)%pred (list2mem m) ]] *
            [[ (A * inum |-> ino)%pred (list2mem ilist) ]]
     POST:r MEMLOG.rep lxp (ActiveTxn mbase m) ms * [[ r = $ (length (IBlocks ino)) ]]
     CRASH  MEMLOG.log_intact lxp mbase
@@ -708,9 +707,9 @@ Module INODE.
 
 
   Theorem igetsz_ok : forall lxp xp inum ms,
-    {< F A mbase m ilist ino bxp,
+    {< F A mbase m ilist ino,
     PRE    MEMLOG.rep lxp (ActiveTxn mbase m) ms *
-           [[ (F * rep bxp xp ilist)%pred (list2mem m) ]] *
+           [[ (F * rep xp ilist)%pred (list2mem m) ]] *
            [[ (A * inum |-> ino)%pred (list2mem ilist) ]]
     POST:r MEMLOG.rep lxp (ActiveTxn mbase m) ms * [[ r = ISize ino ]]
     CRASH  MEMLOG.log_intact lxp mbase
@@ -726,13 +725,13 @@ Module INODE.
   Qed.
 
   Theorem isetsz_ok : forall lxp xp inum sz ms,
-    {< F A mbase m ilist ino bxp,
+    {< F A mbase m ilist ino,
     PRE      MEMLOG.rep lxp (ActiveTxn mbase m) ms *
-             [[ (F * rep bxp xp ilist)%pred (list2mem m) ]] *
+             [[ (F * rep xp ilist)%pred (list2mem m) ]] *
              [[ (A * inum |-> ino)%pred (list2mem ilist) ]]
     POST:ms' exists m' ilist' ino',
              MEMLOG.rep lxp (ActiveTxn mbase m') ms' *
-             [[ (F * rep bxp xp ilist')%pred (list2mem m') ]] *
+             [[ (F * rep xp ilist')%pred (list2mem m') ]] *
              [[ (A * inum |-> ino')%pred (list2mem ilist') ]] *
              [[ ISize ino' = sz ]]
     CRASH  MEMLOG.log_intact lxp mbase
@@ -765,9 +764,9 @@ Module INODE.
 
 
   Theorem iget_ok : forall lxp xp inum off ms,
-    {< F A B mbase m ilist ino a bxp,
+    {< F A B mbase m ilist ino a,
     PRE    MEMLOG.rep lxp (ActiveTxn mbase m) ms *
-           [[ (F * rep bxp xp ilist)%pred (list2mem m) ]] *
+           [[ (F * rep xp ilist)%pred (list2mem m) ]] *
            [[ (A * inum |-> ino)%pred (list2mem ilist) ]] *
            [[ (B * off |-> a)%pred (list2mem (IBlocks ino)) ]]
     POST:r MEMLOG.rep lxp (ActiveTxn mbase m) ms * [[ r = a ]]
@@ -819,14 +818,14 @@ Module INODE.
 
   (* unused *)
   Theorem iput_ok : forall lxp xp inum off a ms,
-    {< F A B mbase m ilist ino bxp,
+    {< F A B mbase m ilist ino,
     PRE      MEMLOG.rep lxp (ActiveTxn mbase m) ms *
-             [[ (F * rep bxp xp ilist)%pred (list2mem m) ]] *
+             [[ (F * rep xp ilist)%pred (list2mem m) ]] *
              [[ (A * inum |-> ino)%pred (list2mem ilist) ]] *
              [[ (B * off |->?)%pred (list2mem (IBlocks ino)) ]]
     POST:ms' exists m' ilist' ino',
              MEMLOG.rep lxp (ActiveTxn mbase m') ms' *
-             [[ (F * rep bxp xp ilist')%pred (list2mem m') ]] *
+             [[ (F * rep xp ilist')%pred (list2mem m') ]] *
              [[ (A * inum |-> ino')%pred (list2mem ilist') ]] *
              [[ (B * off |-> a)%pred (list2mem (IBlocks ino')) ]]
     CRASH    MEMLOG.log_intact lxp mbase
@@ -913,8 +912,8 @@ Module INODE.
              [[  B (list2mem (IBlocks ino)) ]]
     POST:r   exists m', MEMLOG.rep lxp (ActiveTxn mbase m') (snd r) *
             ([[ fst r = false ]] \/
-             [[ fst r = true ]] * exists ilist' ino',
-             [[ (F * rep bxp xp ilist')%pred (list2mem m') ]] *
+             [[ fst r = true ]] * exists ilist' ino' freelist',
+             [[ (F * rep xp ilist' * BALLOC.rep bxp freelist')%pred (list2mem m') ]] *
              [[ (A * inum |-> ino')%pred (list2mem ilist') ]] *
              [[ (B * $ (length (IBlocks ino)) |-> a)%pred (list2mem (IBlocks ino')) ]])
     CRASH    MEMLOG.log_intact lxp mbase
@@ -974,16 +973,16 @@ Module INODE.
   Hint Extern 1 ({{_}} progseq (igrow_indirect _ _ _ _ _ _ _) _) => apply igrow_indirect_ok : prog.
 
   Theorem igrow_ok : forall lxp bxp xp inum a ms,
-    {< F A B mbase m ilist ino,
+    {< F A B mbase m ilist ino freelist,
     PRE      MEMLOG.rep lxp (ActiveTxn mbase m) ms *
              [[ length (IBlocks ino) < blocks_per_inode ]] *
-             [[ (F * rep bxp xp ilist)%pred (list2mem m) ]] *
+             [[ (F * rep xp ilist * BALLOC.rep bxp freelist)%pred (list2mem m) ]] *
              [[ (A * inum |-> ino)%pred (list2mem ilist) ]] *
              [[  B (list2mem (IBlocks ino)) ]]
     POST:r   exists m', MEMLOG.rep lxp (ActiveTxn mbase m') (snd r) *
             ([[ fst r = false ]] \/
-             [[ fst r = true ]] * exists ilist' ino',
-             [[ (F * rep bxp xp ilist')%pred (list2mem m') ]] *
+             [[ fst r = true ]] * exists ilist' ino' freelist',
+             [[ (F * rep xp ilist' * BALLOC.rep bxp freelist')%pred (list2mem m') ]] *
              [[ (A * inum |-> ino')%pred (list2mem ilist') ]] *
              [[ (B * $ (length (IBlocks ino)) |-> a)%pred (list2mem (IBlocks ino')) ]])
     CRASH    MEMLOG.log_intact lxp mbase
@@ -1022,6 +1021,9 @@ Module INODE.
     rewrite inode_set_blocks_get_blocks.
     rewrite <- firstn_app_updN_eq.
     f_equal; auto.
+    Check inode_blocks_length.
+    rewrite inode_blocks_length with (m := (list2mem d0)).
+
     setoid_rewrite inode_blocks_length with (m := (list2mem d0)); inode_bounds.
     rewrite <- nr_direct_elim; auto.
     pred_apply; cancel.
@@ -1052,15 +1054,15 @@ Module INODE.
 
 
   Theorem ishrink_ok : forall lxp bxp xp inum ms,
-    {< F A B mbase m ilist ino,
+    {< F A B mbase m ilist ino freelist,
     PRE      MEMLOG.rep lxp (ActiveTxn mbase m) ms *
              [[ (IBlocks ino) <> nil ]] *
-             [[ (F * rep bxp xp ilist)%pred (list2mem m) ]] *
+             [[ (F * rep xp ilist * BALLOC.rep bxp freelist)%pred (list2mem m) ]] *
              [[ (A * inum |-> ino)%pred (list2mem ilist) ]] *
              [[ (B * $ (length (IBlocks ino) - 1) |->? )%pred (list2mem (IBlocks ino)) ]]
-    POST:ms' exists m' ilist' ino',
+    POST:ms' exists m' ilist' ino' freelist',
              MEMLOG.rep lxp (ActiveTxn mbase m') ms' *
-             [[ (F * rep bxp xp ilist')%pred (list2mem m') ]] *
+             [[ (F * rep xp ilist' * BALLOC.rep bxp freelist')%pred (list2mem m') ]] *
              [[ (A * inum |-> ino')%pred (list2mem ilist') ]] *
              [[  B (list2mem (IBlocks ino')) ]]
     CRASH    MEMLOG.log_intact lxp mbase
